src/Lean/Elab/Tactic/BVDecide/Frontend/BVDecide/ReifiedBVLogical.lean
@@ -31,8 +31,8 @@ def mkEvalExpr (expr : Expr) : M Expr := do
 Construct a `ReifiedBVLogical` from `ReifiedBVPred` by wrapping it as an atom.
 -/
 def ofPred (bvPred : ReifiedBVPred) : M ReifiedBVLogical := do
-  let boolExpr := .literal bvPred.bvPred
-  let expr := mkApp2 (mkConst ``BoolExpr.literal) (mkConst ``BVPred) bvPred.expr
+  let boolExpr := .atom bvPred.bvPred
+  let expr := mkApp2 (mkConst ``BoolExpr.atom) (mkConst ``BVPred) bvPred.expr
   -- important: This must be the same proof as the bvPred one in order for the cache to be correct
   let proof := bvPred.evalsAtAtoms
   return ⟨boolExpr, bvPred.originalExpr, proof, expr⟩
@@ -48,11 +48,11 @@ def boolAtom (t : Expr) : M (Option ReifiedBVLogical) := do
 Build a reified version of the constant `val`.
 -/
 def mkBoolConst (val : Bool) : M ReifiedBVLogical := do
-  let boolExpr := .const val
-  let expr := mkApp2 (mkConst ``BoolExpr.const) (mkConst ``BVPred) (toExpr val)
+  let logicalExpr := .const val
+  let expr := mkApp (mkConst ``BVLogicalExpr.const) (toExpr val)
   -- This is safe because this proof always holds definitionally.
   let proof := pure none
-  return ⟨boolExpr, toExpr val, proof, expr⟩
+  return ⟨logicalExpr, toExpr val, proof, expr⟩
 
 /--
 Construct the reified version of applying the gate in `gate` to `lhs` and `rhs`.
@@ -62,11 +62,10 @@ and `rhs`.
 def mkGate (lhs rhs : ReifiedBVLogical) (lhsExpr rhsExpr : Expr) (gate : Gate) (origExpr : Expr) :
     M ReifiedBVLogical := do
   let congrThm := congrThmOfGate gate
-  let boolExpr := .gate gate lhs.bvExpr rhs.bvExpr
+  let logicalExpr := .gate gate lhs.bvExpr rhs.bvExpr
   let expr :=
-    mkApp4
-      (mkConst ``BoolExpr.gate)
-      (mkConst ``BVPred)
+    mkApp3
+      (mkConst ``BVLogicalExpr.gate)
       (toExpr gate)
       lhs.expr
       rhs.expr
@@ -85,7 +84,7 @@ def mkGate (lhs rhs : ReifiedBVLogical) (lhsExpr rhsExpr : Expr) (gate : Gate) (
       lhsExpr rhsExpr
       lhsEvalExpr rhsEvalExpr
       lhsProof rhsProof
-  return ⟨boolExpr, origExpr, proof, expr⟩
+  return ⟨logicalExpr, origExpr, proof, expr⟩
 where
   congrThmOfGate (gate : Gate) : Name :=
     match gate with
@@ -99,14 +98,14 @@ Construct the reified version of `Bool.not subExpr`.
 This function assumes that `subExpr` is the expression corresponding to `sub`.
 -/
 def mkNot (sub : ReifiedBVLogical) (subExpr : Expr) (origExpr : Expr) : M ReifiedBVLogical := do
-  let boolExpr := .not sub.bvExpr
-  let expr := mkApp2 (mkConst ``BoolExpr.not) (mkConst ``BVPred) sub.expr
+  let logicalExpr := .not sub.bvExpr
+  let expr := mkApp (mkConst ``BVLogicalExpr.not) sub.expr
   let proof := do
     -- This is safe as `not_congr` holds definitionally if the arguments are defeq.
     let some subProof ← sub.evalsAtAtoms | return none
     let subEvalExpr ← ReifiedBVLogical.mkEvalExpr sub.expr
     return mkApp3 (mkConst ``Std.Tactic.BVDecide.Reflect.Bool.not_congr) subExpr subEvalExpr subProof
-  return ⟨boolExpr, origExpr, proof, expr⟩
+  return ⟨logicalExpr, origExpr, proof, expr⟩
 
 /--
 Construct the reified version of `if discrExpr then lhsExpr else rhsExpr`.
@@ -115,11 +114,10 @@ This function assumes that `discrExpr`, lhsExpr` and `rhsExpr` are the correspon
 -/
 def mkIte (discr lhs rhs : ReifiedBVLogical) (discrExpr lhsExpr rhsExpr : Expr) (origExpr : Expr) :
     M ReifiedBVLogical := do
-  let boolExpr := .ite discr.bvExpr lhs.bvExpr rhs.bvExpr
+  let logicalExpr := .ite discr.bvExpr lhs.bvExpr rhs.bvExpr
   let expr :=
-    mkApp4
-      (mkConst ``BoolExpr.ite)
-      (mkConst ``BVPred)
+    mkApp3
+      (mkConst ``BVLogicalExpr.ite)
       discr.expr
       lhs.expr
       rhs.expr
@@ -141,7 +139,7 @@ def mkIte (discr lhs rhs : ReifiedBVLogical) (discrExpr lhsExpr rhsExpr : Expr) 
       discrExpr lhsExpr rhsExpr
       discrEvalExpr lhsEvalExpr rhsEvalExpr
       discrProof lhsProof rhsProof
-  return ⟨boolExpr, origExpr, proof, expr⟩
+  return ⟨logicalExpr, origExpr, proof, expr⟩
 
 end ReifiedBVLogical
 
